CertiGC/verif_mutable_update.v
@@ -1,0 +1,407 @@
+From CertiGraph.CertiGC Require Import
+  env_graph_gc gc_spec forward_lemmas.
+Require Import CertiGraph.graph.graph_model.
+
+Local Open Scope logic.
+
+Lemma graph_rep_interior_field_address: forall g src pos,
+    graph_has_v g src ->
+    0 <= pos < Zlength (raw_fields (vlabel g src)) ->
+    graph_rep g |--
+      !! (interior_address (InteriorVertexPos src pos) g =
+          field_address
+            (tarray int_or_ptr_type (Zlength (make_fields_vals g src)))
+            [ArraySubsc pos] (vertex_address g src)).
+Proof.
+  intros g src pos Hsrc Hpos.
+  sep_apply (graph_rep_vertex_rep g src Hsrc). Intros sh.
+  unfold vertex_rep, vertex_at. Intros.
+  entailer !.
+  unfold interior_address, field_address.
+  rewrite if_true.
+  - reflexivity.
+  - match goal with
+    | Hfc : field_compatible _ [] _ |- _ =>
+        clear -Hfc Hpos;
+        rewrite <- fields_eq_length in Hpos;
+        unfold field_compatible in *; simpl in *; tauto
+    end.
+Qed.
+
+Lemma heap_head_nth_space_O: forall h,
+    heap_head h = nth_space h O.
+Proof.
+  intros h.
+  destruct (heap_head_cons h) as [sp [rest [Hspaces Hhead]]].
+  unfold nth_space. rewrite Hspaces, Hhead. reflexivity.
+Qed.
+
+Lemma generation_data_at__test_order: forall g h gen i j,
+    graph_has_gen g gen ->
+    0 <= i <= available_size h gen ->
+    0 <= j <= available_size h gen ->
+    0 < available_size h gen ->
+    generation_data_at_ g h gen |--
+      denote_tc_test_order
+        (offset_val (WORD_SIZE * i) (gen_start g gen))
+        (offset_val (WORD_SIZE * j) (gen_start g gen)).
+Proof.
+  intros g h gen i j Hgen Hi Hj Hav.
+  unfold generation_data_at_. rewrite data_at__memory_block. Intros.
+  rewrite sizeof_tarray_int_or_ptr by
+    (unfold available_size; apply available_space_range).
+  rewrite isptr_denote_tc_test_order by
+    (apply isptr_offset_val'; apply graph_has_gen_start_isptr; exact Hgen).
+  unfold test_order_ptrs.
+  rewrite sameblock_offset_val by
+    (apply graph_has_gen_start_isptr; exact Hgen).
+  apply andp_right.
+  - eapply derives_trans with
+      (Q := memory_block (nth_sh g gen)
+              (WORD_SIZE * available_size h gen) (gen_start g gen));
+      [cancel|].
+    apply memory_block_weak_valid_pointer;
+      [unfold WORD_SIZE; lia|unfold WORD_SIZE; lia|].
+    unfold nth_sh. apply readable_nonidentity, writable_readable,
+      generation_share_writable.
+  - eapply derives_trans with
+      (Q := memory_block (nth_sh g gen)
+              (WORD_SIZE * available_size h gen) (gen_start g gen));
+      [cancel|].
+    apply memory_block_weak_valid_pointer;
+      [unfold WORD_SIZE; lia|unfold WORD_SIZE; lia|].
+    unfold nth_sh. apply readable_nonidentity, writable_readable,
+      generation_share_writable.
+Qed.
+
+Lemma sem_sub_pi_available_space_minus: forall s,
+    isptr (space_start s) ->
+    force_val
+      (sem_sub_pi int_or_ptr_type Signed
+        (offset_val (WORD_SIZE * available_space s) (space_start s))
+        (Vint (Int.repr 1))) =
+    offset_val (WORD_SIZE * (available_space s - 1)) (space_start s).
+Proof.
+  intros s Hptr. destruct (space_start s); try contradiction. simpl.
+  rewrite ptrofs_of_ints_unfold, ptrofs_mul_repr, Ptrofs.add_commut,
+    Ptrofs.sub_add_l.
+  rewrite ptrofs_sub_repr, Int.signed_repr by rep_lia.
+  rewrite Ptrofs.add_commut. do 3 f_equal. unfold WORD_SIZE. lia.
+Qed.
+
+Lemma align_compatible_int_or_ptr_tptr: forall z,
+    align_compatible_rec cenv_cs int_or_ptr_type z <->
+    align_compatible_rec cenv_cs (tptr int_or_ptr_type) z.
+Proof.
+  intro z; split; intro H.
+  - eapply align_compatible_rec_by_value_inv in H; [|reflexivity].
+    apply align_compatible_rec_by_value with (ch := Mptr);
+      [reflexivity|exact H].
+  - eapply align_compatible_rec_by_value_inv in H; [|reflexivity].
+    apply align_compatible_rec_by_value with (ch := Mptr);
+      [reflexivity|exact H].
+Qed.
+
+Lemma data_at__int_or_ptr_tptr: forall sh p,
+    data_at_ sh int_or_ptr_type p = data_at_ sh (tptr int_or_ptr_type) p.
+Proof.
+  intros. unfold data_at_, field_at_, data_at, field_at.
+  simpl nested_field_type. simpl nested_field_offset. f_equal; f_equal.
+  apply prop_ext. unfold field_compatible. destruct p; simpl; try tauto.
+  rewrite align_compatible_int_or_ptr_tptr. reflexivity.
+Qed.
+
+Lemma data_at_int_or_ptr_tptr: forall sh p v,
+    isptr v ->
+    data_at sh int_or_ptr_type v p =
+    data_at sh (tptr int_or_ptr_type) v p.
+Proof.
+  intros sh p v Hv. unfold data_at, field_at.
+  simpl nested_field_type. simpl nested_field_offset.
+  destruct v; try contradiction.
+  unfold int_or_ptr_type. cbv [Archi.ptr64 log2_sizeof_pointer].
+  f_equal; f_equal. apply prop_ext. unfold field_compatible.
+  destruct p; simpl; try tauto.
+  rewrite align_compatible_int_or_ptr_tptr. reflexivity.
+Qed.
+
+Lemma body_mutable_update:
+  semax_body Vprog Gprog f_mutable_update int_mutable_update_spec.
+Proof.
+  start_function.
+  rename H into Hrecordable.
+  rename H0 into Hghc.
+  rename H1 into Hrhhc.
+  rename H2 into Hloc.
+  rename H3 into Hext.
+  destruct it as [src pos].
+  destruct Hloc as [Hsrc [Hpos [Hmark Htag]]].
+  assert (Hloc: mutable_location_compatible
+                  g (InteriorVertexPos src pos)) by
+    (exact (conj Hsrc (conj Hpos (conj Hmark Htag)))).
+  destruct (mutable_graph_update_exists
+              g (InteriorVertexPos src pos) v Hloc) as [g' Hupd].
+  assert_PROP (valid_int_or_ptr (exterior2val g v)) as Hvalid.
+  { sep_apply (extr_valid_int_or_ptr g v outlier Hext). entailer!. }
+  assert_PROP
+    (interior_address (InteriorVertexPos src pos) g =
+     field_address
+       (tarray int_or_ptr_type (Zlength (make_fields_vals g src)))
+       [ArraySubsc pos] (vertex_address g src)) as Hcell.
+  { sep_apply (graph_rep_interior_field_address g src pos Hsrc Hpos).
+    entailer!. }
+  pose proof
+    (gt_gs_compatible g (pt_heap (ti_heap t_info)) Hghc O
+       (graph_has_gen_O g)) as Hgsc.
+  destruct Hgsc as [Hstart [Hspace_sh Hused]].
+  assert (Hgenstart:
+    gen_start g O =
+    space_start (heap_head (pt_heap (ti_heap t_info)))).
+  { unfold gen_start. rewrite if_true by apply graph_has_gen_O.
+    rewrite heap_head_nth_space_O. exact Hstart. }
+  unfold info_recordable in Hrecordable.
+  unfold before_gc_thread_info_rep, heap_management_rep. Intros.
+  assert_PROP
+    (field_compatible
+       (tarray int_or_ptr_type (available_size (pt_heap (ti_heap t_info)) O))
+       [] (gen_start g O)) as Harray.
+  { gather_SEP (graph_rep g) (heap_unused_rep (pt_heap (ti_heap t_info))).
+    sep_apply
+      (graph_and_heap_rest_data_at_
+         g (pt_heap (ti_heap t_info)) O (graph_has_gen_O g) Hghc).
+    unfold generation_data_at_. entailer!.
+  }
+  assert (Hused_range:
+    0 <= used_space (heap_head (pt_heap (ti_heap t_info))) <=
+    available_space (heap_head (pt_heap (ti_heap t_info)))).
+  { apply used_leq_available. }
+  assert (Halloc_address:
+    field_address0
+      (tarray int_or_ptr_type (available_size (pt_heap (ti_heap t_info)) O))
+      [ArraySubsc (used_space (heap_head (pt_heap (ti_heap t_info))))]
+      (gen_start g O) =
+    offset_val
+      (WORD_SIZE * used_space (heap_head (pt_heap (ti_heap t_info))))
+      (space_start (heap_head (pt_heap (ti_heap t_info))))).
+  { rewrite arr_field_address0.
+    - rewrite Hgenstart. reflexivity.
+    - exact Harray.
+    - unfold available_size. rewrite <- heap_head_nth_space_O. exact Hused_range. }
+  assert (Hlimit_address:
+    field_address0
+      (tarray int_or_ptr_type (available_size (pt_heap (ti_heap t_info)) O))
+      [ArraySubsc (available_space (heap_head (pt_heap (ti_heap t_info))))]
+      (gen_start g O) =
+    offset_val
+      (WORD_SIZE * available_space (heap_head (pt_heap (ti_heap t_info))))
+      (space_start (heap_head (pt_heap (ti_heap t_info))))).
+  { rewrite arr_field_address0.
+    - rewrite Hgenstart. reflexivity.
+    - exact Harray.
+    - unfold available_size. rewrite <- heap_head_nth_space_O. lia. }
+  assert (Hcmp:
+    typed_true tint
+      (force_val
+        (sem_cmp_pp Clt
+          (offset_val
+            (WORD_SIZE * used_space (heap_head (pt_heap (ti_heap t_info))))
+            (space_start (heap_head (pt_heap (ti_heap t_info)))))
+          (offset_val
+            (WORD_SIZE * available_space (heap_head (pt_heap (ti_heap t_info))))
+            (space_start (heap_head (pt_heap (ti_heap t_info)))))))).
+  { rewrite <- Halloc_address, <- Hlimit_address.
+    rewrite ptr_comparison_lt_iff.
+    - exact Hrecordable.
+    - exact Harray.
+    - unfold available_size. rewrite <- heap_head_nth_space_O. exact Hused_range.
+    - unfold available_size. rewrite <- heap_head_nth_space_O. lia.
+    - change (0 < WORD_SIZE). unfold WORD_SIZE. lia.
+    - apply graph_has_gen_start_isptr, graph_has_gen_O.
+  }
+  assert_PROP (isptr ti) as Hti by entailer!.
+  forward.
+  - entailer !. apply isptr_is_pointer_or_null. apply isptr_offset_val'.
+    rewrite <- Hgenstart. apply graph_has_gen_start_isptr, graph_has_gen_O.
+  - forward.
+    + entailer !. apply isptr_is_pointer_or_null. apply isptr_offset_val'.
+      rewrite <- Hgenstart. apply graph_has_gen_start_isptr, graph_has_gen_O.
+    + forward_if True.
+      * sep_apply
+          (graph_and_heap_rest_data_at_
+             g (pt_heap (ti_heap t_info)) O (graph_has_gen_O g) Hghc).
+        sep_apply
+          (generation_data_at__test_order
+             g (pt_heap (ti_heap t_info)) O
+             (used_space (heap_head (pt_heap (ti_heap t_info))))
+             (available_space (heap_head (pt_heap (ti_heap t_info))))).
+        { apply graph_has_gen_O. }
+        { unfold available_size. rewrite <- heap_head_nth_space_O.
+          exact Hused_range. }
+        { unfold available_size. rewrite <- heap_head_nth_space_O. lia. }
+        { unfold available_size. rewrite <- heap_head_nth_space_O. lia. }
+        { rewrite Hgenstart.
+          rewrite !isptr_denote_tc_test_order by
+            (apply isptr_offset_val'; rewrite <- Hgenstart;
+             apply graph_has_gen_start_isptr, graph_has_gen_O).
+          unfold test_order_ptrs.
+          rewrite !sameblock_offset_val by
+            (rewrite <- Hgenstart;
+             apply graph_has_gen_start_isptr, graph_has_gen_O).
+          apply andp_right.
+          - apply sepcon_weak_valid_pointer1.
+            apply andp_left1. apply derives_refl.
+          - apply sepcon_weak_valid_pointer1.
+            apply andp_left2. apply derives_refl. }
+      * forward. entailer!.
+      * exfalso. unfold force_val in Hcmp.
+        unfold typed_true, typed_false in *. congruence.
+      * assert (Hsrc_share:
+          writable_share (nth_sh g (vgeneration src))).
+        { unfold nth_sh. apply generation_share_writable. }
+        sep_apply
+          (graph_rep_mutable_update_ramif
+             g src pos v g' Hloc Hupd).
+        Intros.
+        rewrite Hcell.
+        let p := constr:(field_address
+          (tarray int_or_ptr_type (Zlength (make_fields_vals g src)))
+          [ArraySubsc pos] (vertex_address g src)) in
+        assert_PROP (field_compatible int_or_ptr_type [] p) as Hfield.
+        { entailer!. }
+        assert (Hfield_address:
+          field_address
+            (tarray int_or_ptr_type (Zlength (make_fields_vals g src)))
+            [ArraySubsc pos] (vertex_address g src) =
+          field_address int_or_ptr_type []
+            (field_address
+              (tarray int_or_ptr_type (Zlength (make_fields_vals g src)))
+              [ArraySubsc pos] (vertex_address g src))).
+        { unfold field_address at 2. rewrite if_true by exact Hfield. simpl.
+          symmetry. apply isptr_offset_val_zero. destruct Hfield; assumption. }
+        forward.
+        gather_SEP
+          (field_at (nth_sh g (vgeneration src)) int_or_ptr_type []
+             (exterior2val g v)
+             (field_address
+                (tarray int_or_ptr_type (Zlength (make_fields_vals g src)))
+                [ArraySubsc pos] (vertex_address g src)))
+          (data_at (nth_sh g (vgeneration src)) int_or_ptr_type
+             (exterior2val g v)
+             (field_address
+                (tarray int_or_ptr_type (Zlength (make_fields_vals g src)))
+                [ArraySubsc pos] (vertex_address g src)) -* graph_rep g').
+        replace_SEP 0 (graph_rep g').
+        { entailer !!. apply wand_frame_elim. }
+        forward_call (exterior2val g v).
+        rewrite
+          (heap_remset_rep_mutable_graph_update
+             g (InteriorVertexPos src pos) v g'
+             (pt_heap (ti_heap t_info)) rh Hloc Hupd).
+        assert (Hghc':
+          graph_heap_compatible g' (pt_heap (ti_heap t_info))).
+        { eapply mutable_graph_update_graph_heap_compatible; eassumption. }
+        remember (exterior2val g v) as x eqn:Hx.
+        destruct x; simpl in Hvalid; try contradiction.
+        { forward_if.
+          - contradiction.
+          - forward.
+            assert (Hnptr: ~ isptr (exterior2val g v)).
+            { intro Hp. rewrite <- Hx in Hp. contradiction. }
+            Exists g' t_info rh.
+            unfold decr_info_nursery, mtb_upd_remset_heap.
+            destruct (isptr_dec (exterior2val g v)); [contradiction|].
+            entailer!.
+            unfold before_gc_thread_info_rep, heap_management_rep.
+            cancel. }
+        { forward_if.
+          - assert (Hnursery_ptr:
+              isptr (space_start (heap_head (pt_heap (ti_heap t_info))))).
+            { rewrite <- Hgenstart.
+              apply graph_has_gen_start_isptr, graph_has_gen_O. }
+            forward.
+            forward.
+            simpl force_val.
+            rewrite sem_sub_pi_available_space_minus by exact Hnursery_ptr.
+            forward.
+            assert (Hrecordable0:
+              used_space (nth_space (pt_heap (ti_heap t_info)) O) <
+              available_space (nth_space (pt_heap (ti_heap t_info)) O)).
+            { rewrite <- heap_head_nth_space_O. exact Hrecordable. }
+            sep_apply
+              (heap_unused_rep_incr
+                 g' (pt_heap (ti_heap t_info)) O Hghc'
+                 (graph_has_gen_O g') Hrecordable0).
+            Intros.
+            rewrite data_at__int_or_ptr_tptr.
+            assert (Hspacew:
+              writable_share
+                (space_sh (nth_space (pt_heap (ti_heap t_info)) O))).
+            { rewrite <- Hspace_sh. apply generation_share_writable. }
+            rewrite heap_head_nth_space_O.
+            forward.
+            assert (Hpcell_ptr:
+              isptr
+                (field_address
+                   (tarray int_or_ptr_type
+                     (Zlength (make_fields_vals g src)))
+                   [ArraySubsc pos] (vertex_address g src))).
+            { destruct Hfield. assumption. }
+            rewrite <- data_at_int_or_ptr_tptr by exact Hpcell_ptr.
+            rewrite <- Hcell. unfold interior_address.
+            assert (Haddr:
+              vertex_address g' src = vertex_address g src).
+            { eapply mutable_graph_update_vertex_address; eassumption. }
+            rewrite <- Haddr.
+            sep_apply
+              (remset_rep_upd_int
+                 g' (pt_heap (ti_heap t_info)) O rh src pos Hghc'
+                 (graph_has_gen_O g') Hrhhc Hrecordable0).
+            set (h := pt_heap (ti_heap t_info)) in *.
+            set (hp := ti_heap_p t_info) in *.
+            assert (Hrange0: 0 <= Z.of_nat O < Zlength (spaces h)).
+            { pose proof (spaces_size h) as Hlen.
+              rewrite MAX_SPACES_eq in Hlen. lia. }
+            assert (Htails:
+              tl (spaces (incr_remset_heap h (Z.of_nat O))) =
+              tl (spaces h)).
+            { rewrite spaces_incr_remset_heap_split by exact Hrange0.
+              simpl. destruct (spaces h); reflexivity. }
+            assert (Htoken:
+              ti_token_rep h hp =
+              ti_token_rep (incr_remset_heap h (Z.of_nat O)) hp).
+            { apply ti_token_rep_weak_heap_relation.
+              apply incr_remset_heap_whr. }
+            Exists g'
+              (Build_thread_info
+                 hp
+                 (build_compatible_heap
+                    (incr_remset_heap h (Z.of_nat O)))
+                 (ti_args t_info) (arg_size t_info)
+                 (ti_frames t_info) (ti_nalloc t_info))
+              (upd_remset_heap
+                 (RemSetInterior (InteriorVertexPos src pos)) rh O).
+            unfold decr_info_nursery, mtb_upd_remset_heap.
+            destruct (isptr_dec (Vptr b i)) as [Hptr | Hnptr].
+            2: { exfalso. apply Hnptr. exact I. }
+            entailer!.
+            unfold before_gc_thread_info_rep, heap_management_rep.
+            simpl pt_heap. rewrite heap_head_nth_space_O.
+            rewrite irh_used_space, irh_space_start, irh_total_space.
+            pose proof
+              (irh_available_space_same h O Hrange0 Hrecordable0)
+              as Havail.
+            pose proof Htails as Htails'.
+            pose proof Htoken as Htoken'.
+            cbn in Havail, Htails', Htoken'.
+            rewrite Htoken'.
+            rewrite Havail, Htails'.
+            unfold ti_fp. simpl ti_frames. cancel.
+            cbv [Vptrofs Archi.ptr64].
+            unfold data_at, field_at.
+            simpl nested_field_type. simpl nested_field_offset.
+            simpl ti_heap_p. cancel. apply derives_refl.
+          - match goal with
+            | Hfalse : Int.repr 1 = Int.zero |- _ =>
+                apply Int.one_not_zero in Hfalse; contradiction
+            end. }
+Qed.
